big changes: sets of formulas, countability, lindenbaum, tautologies

hybrid/Form.lean
@@ -1,3 +1,5 @@
+import Mathlib.Data.Set.Basic
+import Mathlib.Data.Nat.Parity
 import Hybrid.Util
 
 section Basics
@@ -12,6 +14,39 @@ section Basics
   structure NOM where
     letter : Nat
   deriving DecidableEq, Repr
+
+  instance : Max PROP where
+    max := λ p => λ q => ite (p.letter > q.letter) p q
+  instance svarmax : Max SVAR where
+    max := λ x => λ y => ite (x.letter > y.letter) x y
+  instance : Max NOM where
+    max := λ i => λ j => ite (i.letter > j.letter) i j
+
+
+  instance : OfNat SVAR n    where
+    ofNat := SVAR.mk n
+  instance : OfNat NOM n     where
+    ofNat := NOM.mk  n
+  instance : Coe SVAR Nat  := ⟨SVAR.letter⟩
+--  instance : Coe NOM Nat   := ⟨NOM.letter⟩
+  instance : Coe Nat SVAR  := ⟨SVAR.mk⟩   
+--  instance : Coe Nat NOM   := ⟨NOM.mk⟩   
+  instance SVAR.le : LE SVAR         where
+    le    := λ x => λ y =>  x.letter ≤ y.letter
+  instance : LT SVAR         where
+    lt    := λ x => λ y =>  x.letter < y.letter
+  instance NOM.le : LE NOM         where
+    le    := λ x => λ y =>  x.letter ≤ y.letter
+  instance  : HAdd SVAR Nat SVAR where
+    hAdd  := λ x => λ n => SVAR.mk (x.letter + n)
+  instance : HAdd NOM Nat NOM where
+    hAdd  := λ x => λ n => NOM.mk (x.letter + n)
+  instance : HMul NOM Nat NOM where
+    hMul  := λ x => λ n => NOM.mk (x.letter * n)
+  instance : HMul Nat NOM NOM where
+    hMul  := λ n => λ x => NOM.mk (x.letter * n)
+  instance : HMul NOM ℕ ℕ where
+    hMul  := λ x => λ n => x.letter * n
 
   inductive Form where
     -- atomic formulas:
@@ -32,10 +67,12 @@ section Basics
   @[simp]
   def Form.conj     : Form → Form → Form := λ φ => λ ψ => Form.neg (Form.impl φ (Form.neg ψ))
   @[simp]
+  def Form.iff      : Form → Form → Form := λ φ => λ ψ => Form.conj (Form.impl φ ψ) (Form.impl ψ φ) 
+  @[simp]
   def Form.disj     : Form → Form → Form := λ φ => λ ψ => Form.impl (Form.neg φ) ψ
   @[simp]
   def Form.diamond  : Form → Form := λ φ => Form.neg (Form.box (Form.neg φ))
-  @[simp]
+  @[simp,match_pattern]
   def Form.bind_dual: SVAR → Form → Form := λ x => λ φ => Form.neg (Form.bind x (Form.neg φ))
 
   instance : Coe PROP Form  := ⟨Form.prop⟩
@@ -45,112 +82,61 @@ section Basics
   infixr:60 "⟶" => Form.impl
   infixl:65 "⋀" => Form.conj
   infixl:65 "⋁" => Form.disj
-  prefix:70 "∼" => Form.neg
   prefix:100 "□" => Form.box
   prefix:100 "◇ " => Form.diamond
   notation:120 "all " x ", " φ => Form.bind x φ
   notation:120 "ex " x ", " φ => Form.bind_dual x φ
+  prefix:170 "∼" => Form.neg
+  infixr:60 "⟷" => Form.iff
   notation "⊥"  => Form.bttm
 
-  @[simp]
-  def conjunction (Γ : List Form) : Form :=
-  match Γ with
+  def conjunction (Γ : Set Form) (L : List Γ) : Form :=
+  match L with
     | []     => ⊥ ⟶ ⊥
-    | h :: t => h ⋀ conjunction t
-  
-  @[simp]
-  theorem on_conj : (h ⋀ conjunction t) = (conjunction (h :: t)) := by
-    rw [conjunction]
+    | h :: t => h.val ⋀ conjunction Γ t
+
+  def Form.new_var  : Form → SVAR
+  | .svar x   => x+1
+  | .impl ψ χ => max (ψ.new_var) (χ.new_var)
+  | .box  ψ   => ψ.new_var
+  | .bind x ψ => max (x+1) (ψ.new_var)
+  | _         => 0
+
+  def Form.new_nom  : Form → NOM
+  | .nom  i   => i+1
+  | .impl ψ χ => max (ψ.new_nom) (χ.new_nom)
+  | .box  ψ   => ψ.new_nom
+  | .bind _ ψ => ψ.new_nom
+  | _         => 0
 
 end Basics
 
-section Variables
-  instance : LT SVAR where
-    lt := λ x y => x.letter < y.letter  
-  instance : HAdd SVAR Nat SVAR where
-    hAdd := λ v n => { letter := v.letter + n }
-  instance : HAdd Nat SVAR SVAR where
-    hAdd := λ n v => { letter := v.letter + n }
-  instance (x y : SVAR) : Decidable (x < y) :=
-      dite (x.letter < y.letter) (λ tr => isTrue tr) (λ fls => isFalse fls)
-
-  def max_svar (l : List SVAR) : SVAR :=
-    match l with
-      | []     => {letter := (default : Nat)}
-      | h :: t => max h (max_svar t)
-  
-  def list_vars (φ : Form) : List SVAR :=
-    match φ with
-    | Form.svar x   => [x]
-    | Form.impl φ ψ => (list_vars φ) ++ (list_vars ψ)
-    | Form.box φ    => list_vars φ
-    | Form.bind _ φ => list_vars φ
-    | _             => []
-
-  def occurs (x : SVAR) (φ : Form) : Bool := (list_vars φ).contains x
-
-  def get_fresh_var (φ : Form) : SVAR := {letter := (max_svar (list_vars φ)).letter + 1}
-end Variables
-
 section Substitutions
-  def is_free (x : SVAR) (φ : Form) : Prop :=
+  def occurs (x : SVAR) (φ : Form) : Bool :=
     match φ with
-    | Form.bttm     => True
-    | Form.prop _   => True
-    | Form.svar _   => True
-    | Form.nom  _   => True
-    | Form.impl φ ψ => (is_free x φ) ∨ (is_free x ψ)
+    | Form.bttm     => false
+    | Form.prop _   => false
+    | Form.svar y   => x = y
+    | Form.nom  _   => false
+    | Form.impl φ ψ => (occurs x φ) || (occurs x ψ)
+    | Form.box  φ   => occurs x φ
+    | Form.bind _ φ => occurs x φ
+
+  def is_free (x : SVAR) (φ : Form) : Bool :=
+    match φ with
+    | Form.bttm     => false
+    | Form.prop _   => false
+    | Form.svar y   => x == y
+    | Form.nom  _   => false
+    | Form.impl φ ψ => (is_free x φ) || (is_free x ψ)
     | Form.box  φ   => is_free x φ
-    | Form.bind y φ => ite (y = x) False (is_free x φ)
+    | Form.bind y φ => (y != x) && (is_free x φ)
 
-  instance DecidableIsFree : Decidable (is_free x φ) := by
-    match φ with
-    | Form.bttm     => exact isTrue trivial
-    | Form.prop _   => exact isTrue trivial
-    | Form.svar _   => exact isTrue trivial
-    | Form.nom  _   => exact isTrue trivial
-    | Form.box  φ   => exact (@DecidableIsFree x φ)
-    | Form.impl φ ψ =>
-        have ih_1 := @DecidableIsFree x φ
-        have ih_2 := @DecidableIsFree x ψ
-        match ih_1 with
-        | isTrue p  => exact isTrue (Or.inl p)
-        | isFalse p =>
-            match ih_2 with
-            | isTrue  q => exact isTrue (Or.inr q)
-            | isFalse q => exact isFalse (negated_disjunction.mpr ⟨p, q⟩)
-    | Form.bind y φ =>
-        have ih := @DecidableIsFree x φ
-        match ih with
-        | isTrue p =>
-            exact dite (y = x) (λ eq =>
-                    isFalse (show ¬is_free x (all y, φ) by
-                      intro t
-                      unfold is_free at t
-                      rw [if_pos eq] at t
-                      exact t)
-                    )
-                  (λ neq =>
-                    isTrue (show is_free x (all y, φ) by
-                      unfold is_free
-                      rw [if_neg neq]
-                      assumption)
-                    )
-        | isFalse p =>
-            exact dite (y = x) (λ eq =>
-                    isFalse (show ¬is_free x (all y, φ) by
-                      intro t
-                      unfold is_free at t
-                      rw [if_pos eq] at t
-                      exact t)
-                    )
-                  (λ neq =>
-                    isFalse (show ¬is_free x (all y, φ) by
-                      unfold is_free
-                      rw [if_neg neq]
-                      assumption)
-                    )
+  #eval is_free (SVAR.mk 0) ⊥
+  #eval is_free (SVAR.mk 0) (all SVAR.mk 0, ⊥)
 
+  def is_bound (x : SVAR) (φ : Form) := (occurs x φ) && !(is_free x φ)
+  
   -- conventions for substitutions can get confusing
   -- "φ[s // x], the formula obtained by substituting s for all *free* occurrences of x in φ"
   -- for reference: Blackburn 1998, pg. 628
@@ -174,15 +160,17 @@ section Substitutions
     | Form.box  φ   => □ (subst_nom φ s x)
     | Form.bind y φ => ite (x = y) (Form.bind y φ) (Form.bind y (subst_nom φ s x))
 
-  def is_substable (φ : Form) (s : SVAR) (x : SVAR) : Prop :=
+  def is_substable (φ : Form) (y : SVAR) (x : SVAR) : Bool :=
     match φ with
-    | Form.bttm     => True
-    | Form.prop _   => True
-    | Form.svar _   => True
-    | Form.nom  _   => True
-    | Form.impl φ ψ => (is_substable φ s x) ∧ (is_substable ψ s x)
-    | Form.box  φ   => is_substable φ s x
-    | Form.bind y φ => ite (¬is_free x φ) True (ite (s ≠ y) (is_substable φ s x) False)
+    | Form.bttm     => true
+    | Form.prop _   => true
+    | Form.svar _   => true
+    | Form.nom  _   => true
+    | Form.impl φ ψ => (is_substable φ y x) && (is_substable ψ y x)
+    | Form.box  φ   => is_substable φ y x
+    | Form.bind z φ =>
+        if (is_free x φ == false) then true
+        else z != y && is_substable φ y x
     -- all s, s ⟶ (all x, x)  : safe,   substitution won't do anything
     -- all x, x                : safe,   substitution won't do anything
     -- all y, y ⟶ x           : safe,   result will be   all y, y ⟶ s
@@ -195,53 +183,666 @@ section Substitutions
   notation:150 φ "[" s "//" x "]" => subst_svar φ s x
   notation:150 φ "[" s "//" x "]" => subst_nom  φ s x
 
-  theorem preserve_boundness {φ : Form} {x v : SVAR} : ¬is_free x φ → (¬ is_free x (all v, φ)) := by
-    intro h1 h2
-    simp [is_free] at h2
-    by_cases v_x : v = x
-    . simp [v_x] at h2
-    . simp [v_x] at h2
-      exact show False from h1 h2
+  #eval is_substable (all SVAR.mk 0, all SVAR.mk 1, SVAR.mk 0) (SVAR.mk 1) (SVAR.mk 0)  
+  #eval subst_svar (all SVAR.mk 0, all SVAR.mk 1, SVAR.mk 0) (SVAR.mk 1) (SVAR.mk 0)
+  #eval occurs 1 (all 0, all 1, SVAR.mk 0)
 
-  theorem subst_bound_var {φ : Form} {x y : SVAR} (h : ¬is_free x φ) : (φ[y // x] = φ) := by
+  lemma new_var_gt      : occurs x φ → x < φ.new_var   := by
     induction φ with
-    | svar v =>
-        by_cases x_v : x = v
-        . conv at h => rhs ; simp [is_free]
-          simp at h
-        . simp [subst_svar, x_v]
-    | impl ψ χ ind₁ ind₂ =>
-        simp [is_free, negated_disjunction] at h
-        conv =>
-          lhs
-            simp [subst_svar]
-            congr
-            . rw [ind₁ h.left]
-            . rw [ind₂ h.right]
-    | box ψ ind =>
-        simp [is_free] at h
-        simp [subst_svar]
-        apply ind
+    | svar y          =>
+        simp [occurs, Form.new_var, -implication_disjunction]
+        intro h
+        rw [h]
+        exact Nat.lt_succ_self y.letter
+    | impl ψ χ ih1 ih2 =>
+        simp only [occurs, Form.new_var, Bool.or_eq_true, max]
+        intro h
+        apply Or.elim h
+        . intro ha
+          clear ih2 h
+          have ih1 := ih1 ha
+          by_cases hc : (Form.new_var ψ).letter > (Form.new_var χ).letter
+          . simp [hc]
+            assumption
+          . simp [hc]
+            simp at hc 
+            exact Nat.lt_of_lt_of_le ih1 hc
+        . intro hb
+          clear ih1 h
+          have ih2 := ih2 hb
+          by_cases hc : (Form.new_var ψ).letter > (Form.new_var χ).letter
+          . simp [hc]
+            simp at hc
+            exact Nat.lt_trans ih2 hc
+          . simp [hc]
+            assumption
+    | box ψ ih      =>
+        simp only [occurs, Form.new_var]
         assumption
-    | bind v ψ ind =>
-        simp [is_free] at h
-        by_cases v_x : v = x
-        . conv =>
-            lhs
-              simp [subst_svar, v_x]
-          simp [v_x]
-        . simp [is_free, v_x] at h
-          conv =>
-            lhs
-              simp [subst_svar, Ne.symm v_x]
-              rhs rw [ind h]
-      | _ => simp [subst_svar]
+    | bind y ψ ih   =>
+        simp only [occurs, Form.new_var, max]
+        intro h
+        have ih := ih h
+        by_cases hc : (y + 1).letter > (Form.new_var ψ).letter
+        . simp [hc]
+          simp at hc
+          exact Nat.lt_trans ih hc
+        . simp [hc]
+          assumption
+    | _ => simp [occurs]
 
-  theorem not_bound_when_quantified : ¬is_free x (all x, φ) := by
+  lemma new_var_is_new  : occurs (φ.new_var) φ = false := by
+    rw [←Bool.eq_false_eq_not_eq_true]
     intro h
-    simp [is_free] at h
+    have a := new_var_gt h
+    have b := Nat.lt_irrefl φ.new_var.letter
+    exact b a
+  
+  lemma ge_new_var_is_new (h : x ≥ φ.new_var) : occurs x φ = false := by
+    rw [←Bool.eq_false_eq_not_eq_true]
+    intro habs
+    have := new_var_gt habs
+    have a := Nat.lt_of_le_of_lt h this
+    have b := Nat.lt_irrefl φ.new_var.letter
+    exact b a
+  
+  lemma notfreeset {Γ : Set Form} (L : List Γ) (hyp : ∀ ψ : Γ, is_free x ψ = false) : is_free x (conjunction Γ L) = false := by
+    induction L with
+    | nil         =>
+        simp only [conjunction, is_free]
+    | cons h t ih =>
+        simp only [is_free, Bool.or_false, Bool.or_eq_false_eq_eq_false_and_eq_false]
+        apply And.intro
+        . exact hyp h
+        . exact ih
+
+  lemma notfree_after_subst {φ : Form} {x y : SVAR} (h : x ≠ y) : is_free x (φ[y // x]) = false := by
+    induction φ with
+    | svar z   =>
+        by_cases xz : x = z
+        . simp [subst_svar, if_pos xz, is_free, h]
+        . simp [subst_svar, if_neg xz, is_free, xz]
+    | impl _ _ ih1 ih2 =>
+        simp [subst_svar, is_free, ih1, ih2]
+    | box _ ih    =>
+        simp [subst_svar, is_free, ih]
+    | bind z _ ih =>
+        by_cases xz : x = z
+        . simp [subst_svar, xz, is_free]
+        . simp [subst_svar, if_neg xz, is_free, ih]
+    | _        => simp only [is_free]
+
+  lemma notocc_beforeafter_subst {φ : Form} {x y : SVAR} (h : occurs x φ = false) : occurs x (φ[y // x]) = false := by
+    induction φ with
+    | svar z   =>
+        by_cases xz : x = z
+        <;> simp [subst_svar, if_pos xz, xz, occurs, h] at *
+    | impl _ _ ih1 ih2 =>
+        simp [subst_svar, occurs, not_or, ih1, ih2, -implication_disjunction] at *
+        exact ⟨ih1 h.left, ih2 h.right⟩ 
+    | box _ ih    =>
+        simp [subst_svar, occurs, ih, -implication_disjunction] at *
+        exact ih h
+    | bind z ψ ih =>
+        by_cases xz : x = z
+        . simp [subst_svar, xz, occurs] at *
+          exact h
+        . simp [subst_svar, if_neg xz, occurs, ih, xz, h, -implication_disjunction] at *
+          exact ih h
+    | _        => simp only [occurs]
+
+  lemma notoccursbind : occurs x φ = false → occurs x (all v, φ) = false := by
+    simp [occurs]
+
+  lemma notoccurs_notfree : (occurs x φ = false) → (is_free x φ = false) := by
+    induction φ with
+    | svar _ => simp [occurs, is_free]
+    | impl _ _ ih1 ih2 =>
+        intro h
+        simp [occurs] at h
+        simp [is_free, ih1, ih2, h]
+    | box _ ih        =>
+        intro h
+        rw [occurs] at h
+        simp [is_free, ih, h]
+    | bind _ _ ih     =>
+        intro h
+        rw [occurs] at h
+        simp [is_free, ih, h]
+    | _ => 
+        intro h
+        rfl
+
+  lemma preserve_notfree {φ : Form} (x v : SVAR) : (is_free x φ = false) → (is_free x (all v, φ) = false) := by
+    intro h
+    simp only [is_free, h, Bool.and_false]
+
+  -- φ = all x, all y, x
+  -- φ[y // x] = φ:                 (x is bound in φ)
+  #eval (all SVAR.mk 0, all SVAR.mk 1, SVAR.mk 0)[SVAR.mk 1 // SVAR.mk 0]
+  --  but is_subst φ y x = false:   (x occurs free in the scope of y)
+  #eval is_substable (all SVAR.mk 0, all SVAR.mk 1, SVAR.mk 0) (SVAR.mk 1) (SVAR.mk 0)
+  lemma subst_notfree_var {φ : Form} {x y : SVAR} (h : is_free x φ = false) : (φ[y // x] = φ) ∧ (occurs x φ = false → is_substable φ y x) := by
+    induction φ with
+    | svar z =>
+        by_cases heq : x = z
+        . simp only [is_free, heq, beq_self_eq_true] at h 
+        . simp only [subst_svar, heq, ite_false, occurs, is_substable]
+    | impl ψ χ ih1 ih2 =>
+        simp only [is_free, Bool.or_eq_false_eq_eq_false_and_eq_false] at h 
+        apply And.intro
+        . simp [subst_svar, h, ih1, ih2]
+        . intro nocc
+          simp only [occurs, Bool.or_eq_false_eq_eq_false_and_eq_false] at nocc 
+          simp [is_substable, h, nocc, ih1, ih2]
+    | box ψ ih  =>
+        rw [is_free] at h
+        apply And.intro
+        . simp [subst_svar, ih, h]
+        . intro nocc
+          rw [occurs] at nocc
+          simp [is_substable, ih, nocc, h]
+    | bind z ψ ih =>
+        apply And.intro
+        . by_cases heq : x = z
+          . rw [←heq, subst_svar, if_pos (Eq.refl x)]
+          . simp only [is_free, bne, Bool.and_eq_false_eq_eq_false_or_eq_false, Bool.not_eq_false', beq_iff_eq,
+            Ne.symm heq, false_or] at h 
+            simp [subst_svar, heq, ih, h]
+        . intro nocc
+          rw [occurs] at nocc
+          simp [is_substable, notoccurs_notfree, nocc]
+    | _   =>
+        simp [subst_svar, is_substable]
+
+    lemma rereplacement (φ : Form) (x y : SVAR) (h1 : occurs y φ = false) (h2 : is_substable φ y x) : (is_substable (φ[y // x]) x y) ∧ φ[y // x][x // y] = φ := by
+      induction φ with
+      | svar z =>
+          simp [occurs] at h1
+          by_cases xz : x = z
+          repeat simp [subst_svar, xz, h1, is_substable]
+      | impl ψ χ ih1 ih2 =>
+          simp only [occurs, Bool.or_eq_false_eq_eq_false_and_eq_false] at h1 
+          simp only [is_substable, Bool.and_eq_true] at h2
+          simp [subst_svar, ih1, ih2, h1, h2, is_substable]
+      | box ψ ih =>
+          simp only [occurs] at h1
+          simp only [is_substable] at h2
+          simp [subst_svar, ih, h1, h2, is_substable]
+      | bind z ψ ih =>
+          by_cases yz : y = z
+          . rw [←yz]
+            rw [←yz] at h1
+
+            simp only [is_substable, beq_iff_eq, ←yz, bne_self_eq_false, Bool.false_and, ite_eq_left_iff,
+              Bool.not_eq_false, implication_disjunction, Bool.not_eq_true, or_false] at h2 
+            have h2 := @preserve_notfree ψ x y h2
+            simp [subst_notfree_var, h2]
+
+            have := @subst_notfree_var (all y, ψ) y x (notoccurs_notfree h1)
+            simp [@subst_notfree_var (all y, ψ) y x, notoccurs_notfree, h1]
+          . by_cases xz : x = z
+            . have : is_free x (all x, ψ) = false := by simp [is_free]
+              rw [←xz] at h1
+              simp [←xz, subst_notfree_var, this, notoccurs_notfree, h1]
+            . simp only [occurs] at h1
+              simp [subst_svar, xz, yz]
+              by_cases xfree : is_free x ψ
+              . simp [is_substable, xfree, Ne.symm yz, bne] at h2
+                simp [ih, h1, h2, is_substable, bne, Ne.symm xz]
+              . rw [show (¬is_free x ψ = true ↔ is_free x ψ = false) by simp] at xfree
+                simp [subst_notfree_var, xfree, is_substable, (notoccurs_notfree h1)]
+      | _     =>
+          apply And.intro
+          repeat rfl
+  
+  lemma subst_self_is_self (φ : Form) (x : SVAR) : φ [x // x] = φ := by
+    induction φ with
+    | svar y   =>
+        by_cases xy : x = y
+        . rw [subst_svar, if_pos xy, xy]
+        . rw [subst_svar, if_neg xy]
+    | impl φ ψ ih1 ih2 =>
+        rw [subst_svar, ih1, ih2]
+    | box  φ ih  =>
+        rw [subst_svar, ih]
+    | bind y φ ih =>
+        by_cases xy : x = y
+        . rw [subst_svar, if_pos xy]
+        . rw [subst_svar, if_neg xy, ih]
+    | _        => rfl
 
 end Substitutions
+
+section NominalSubstitution
+
+  def Form.nominals : Form → List NOM
+  | .nom a      => [a]
+  | .impl φ ψ   => φ.nominals ++ ψ.nominals
+  | .box φ      => φ.nominals
+  | .bind _ φ   => φ.nominals
+  | _           => []
+
+  def nom_subst_nom : Form → NOM → NOM → Form
+  | .nom a, i, j     => if a = j then i else a
+  | .impl φ ψ, i, j  => nom_subst_nom φ i j ⟶ nom_subst_nom ψ i j
+  | .box φ, i, j     => □ nom_subst_nom φ i j
+  | .bind y φ, i, j  => all y, nom_subst_nom φ i j
+  | φ, _, _          => φ
+
+  def nom_subst_svar : Form → SVAR → NOM → Form
+  | .nom a, i, j     => if a = j then i else a
+  | .impl φ ψ, i, j  => nom_subst_svar φ i j ⟶ nom_subst_svar ψ i j
+  | .box φ, i, j     => □ nom_subst_svar φ i j
+  | .bind y φ, i, j  => all y, nom_subst_svar φ i j
+  | φ, _, _          => φ
+
+  notation:150 φ "[" i "//" a "]" => nom_subst_nom φ i a
+  notation:150 φ "[" i "//" a "]" => nom_subst_svar φ i a
+
+  def nom_occurs : NOM → Form → Bool
+  | i, .nom j    => i = j
+  | i, .impl ψ χ => (nom_occurs i ψ) || (nom_occurs i χ)
+  | i, .box ψ    => nom_occurs i ψ
+  | i, .bind _ ψ => nom_occurs i ψ
+  | _, _         => false
+
+  def Form.list_noms : Form → List NOM := λ φ =>
+    loop φ.new_nom.letter φ
+  where
+    loop : Nat → Form → List NOM
+    | 0, _     =>      []
+    | n+1, φ   => ite (nom_occurs ⟨n⟩ φ) (⟨n⟩ :: loop n φ) (loop n φ)
+
+  def Form.dbl_list_noms : Form → List NOM := λ φ =>
+    loop φ.new_nom.letter φ
+  where
+    loop : Nat → Form → List NOM
+    | 0, _     =>      []
+    | n+1, φ   =>      ite (nom_occurs ⟨n⟩ φ) (⟨2*n⟩ :: loop n φ) (loop n φ)
+  
+  #eval (NOM.mk 2 ⋁ NOM.mk 3 ⋁ NOM.mk 4).list_noms
+  #eval List.take 9 (NOM.mk 2 ⋁ NOM.mk 3 ⋁ NOM.mk 4).dbl_list_noms
+
+--  theorem dream {φ : Form} (h1 : (h₁ :: t₁) = φ.double_list_noms) (h2 : (h₂ :: t₂) = φ.list_noms)
+
+  def Form.bulk_subst : Form → List NOM → List NOM → Form
+  | φ, h₁ :: t₁, h₂ :: t₂ => bulk_subst (φ[h₁ // h₂]) t₁ t₂
+  | φ, _, []    =>  φ
+  | φ, [], _    =>  φ
+
+  def Form.dbl : Form → Form := λ φ => φ.bulk_subst φ.dbl_list_noms φ.list_noms
+
+  #eval (NOM.mk 2 ⟶ NOM.mk 3 ⟶ NOM.mk 4).dbl
+
+  lemma new_nom_gt      : nom_occurs i φ → i.letter < φ.new_nom.letter   := by
+    induction φ with
+    | nom i          =>
+        simp [nom_occurs, Form.new_nom, -implication_disjunction]
+        intro h
+        rw [h]
+        exact Nat.lt_succ_self i.letter
+    | impl ψ χ ih1 ih2 =>
+        simp only [nom_occurs, Form.new_nom, Bool.or_eq_true, max]
+        intro h
+        apply Or.elim h
+        . intro ha
+          clear ih2 h
+          have ih1 := ih1 ha
+          by_cases hc : (Form.new_nom ψ).letter > (Form.new_nom χ).letter
+          . simp [hc]
+            assumption
+          . simp [hc]
+            simp at hc 
+            exact Nat.lt_of_lt_of_le ih1 hc
+        . intro hb
+          clear ih1 h
+          have ih2 := ih2 hb
+          by_cases hc : (Form.new_nom ψ).letter > (Form.new_nom χ).letter
+          . simp [hc]
+            simp at hc
+            exact Nat.lt_trans ih2 hc
+          . simp [hc]
+            assumption
+    | box      =>
+        assumption
+    | bind     =>
+        assumption
+    | _ => simp [nom_occurs]
+
+  lemma new_nom_is_nom  : nom_occurs (φ.new_nom) φ = false := by
+    rw [←Bool.eq_false_eq_not_eq_true]
+    intro h
+    have a := new_nom_gt h
+    have b := Nat.lt_irrefl φ.new_nom.letter
+    exact b a
+  
+  lemma ge_new_nom_is_new (h : x ≥ φ.new_nom) : nom_occurs x φ = false := by
+    rw [←Bool.eq_false_eq_not_eq_true]
+    intro habs
+    have := new_nom_gt habs
+    have a := Nat.lt_of_le_of_lt h this
+    have b := Nat.lt_irrefl φ.new_nom.letter
+    exact b a
+
+/-
+  theorem all_lt_list_noms {φ : Form} : ∀ n, n < φ.new_nom.letter → ⟨n⟩ ∈ φ.list_noms := by
+    rw [Form.list_noms]
+    induction φ.new_nom.letter with
+    | zero => simp
+    | succ n ih =>
+        intro i i_lt
+        simp [Form.list_noms.loop] at ih ⊢
+        apply Or.elim (ih i)
+        . intro n_le
+          apply Or.inl
+          apply Nat.le_antisymm
+          apply Nat.lt_add_one_iff.mp
+          assumption
+          assumption
+        . clear i_lt ih
+          intro hmem
+          apply Or.inr
+          assumption
+
+  theorem all_lt_list_noms' {φ : Form} : ∀ n, ⟨n⟩ ∈ φ.list_noms ↔ n < φ.new_nom.letter := by
+    intro n
+    apply Iff.intro
+    . rw [Form.list_noms]
+      induction φ.new_nom.letter with
+      | zero    => simp only [Form.list_noms.loop]; intro; contradiction
+      | succ m ih =>
+          simp [Form.list_noms.loop, -implication_disjunction]
+          intro disj
+          apply Or.elim disj
+          . intro
+            simp [*]
+          . intro
+            simp [*, Nat.lt_succ_of_lt] at *
+    . exact all_lt_list_noms n
+-/
+
+  -- bit ugly but it works
+  theorem occurs_list_noms : nom_occurs i φ ↔ i ∈ φ.list_noms := by
+    rw [Form.list_noms]
+    apply Iff.intro
+    . intro h
+      have := new_nom_gt h
+      revert this
+      induction φ.new_nom.letter with
+      | zero => simp
+      | succ n ih =>
+          intro h2
+          rw [Form.list_noms.loop]
+          split
+          . simp
+            by_cases heq : i.letter = n
+            . apply Or.inl
+              rw [NOM.mk.injEq]
+              assumption
+            . simp [Nat.lt_succ_iff_lt_or_eq, heq] at h2
+              apply Or.inr; apply ih; assumption
+          . apply ih
+            have : ¬i.letter = n := by
+                intro habs
+                have : i = {letter := n} := by rw [NOM.mk.injEq, habs]
+                simp [*] at *
+            simp [Nat.lt_succ_iff_lt_or_eq, this] at h2
+            assumption
+    . induction φ.new_nom.letter with
+      | zero => simp [Form.list_noms.loop]
+      | succ n ih =>
+          intro h
+          simp [Form.list_noms.loop] at h
+          split at h
+          . simp at h
+            apply Or.elim h
+            . intro; simp [*]
+            . exact ih
+          . apply ih; assumption
+
+  theorem list_noms_subst {old new : NOM} : i ∈ (φ[new // old]).list_noms → ((i ∈ φ.list_noms ∧ i ≠ old) ∨ i = new) := by
+    --rw [all_lt_list_noms', all_lt_list_noms']
+    rw [←occurs_list_noms, ←occurs_list_noms]
+    intro h
+    induction φ with
+    | nom j =>
+        simp [nom_subst_nom] at h
+        split at h
+        . simp [nom_occurs] at h; apply Or.inr; assumption
+        . apply Or.inl
+          apply And.intro
+          . assumption
+          . simp [nom_occurs] at h
+            rw [h]
+            assumption
+    | impl ψ χ ih1 ih2 =>
+        simp [nom_occurs] at h ⊢
+        apply Or.elim h
+        . intro hyp
+          apply Or.elim (ih1 hyp)
+          . intro hl
+            simp [hl]
+          . intro hr
+            simp [hr]
+        . intro hyp
+          apply Or.elim (ih2 hyp)
+          . intro hl
+            simp [hl]
+          . intro hr
+            simp [hr]
+    | box ψ ih =>
+        simp [nom_occurs] at h
+        exact ih h
+    | bind _ ψ ih =>
+        simp [nom_occurs] at h
+        exact ih h
+    | _     => simp [nom_occurs] at h
+
+  theorem occ_bulk {l_new l_old : List NOM} {φ : Form} (eq_len : l_new.length = l_old.length) : nom_occurs i (φ.bulk_subst l_new l_old) → ((i ∈ φ.list_noms ∧ i ∉ l_old) ∨ i ∈ l_new) := by
+    intro h
+    induction l_new generalizing φ l_old with
+    | nil => cases l_old <;> simp [Form.bulk_subst] at *; repeat exact occurs_list_noms.mp h
+    | cons h_new t_new ih =>
+        cases l_old with
+        | nil =>
+            simp [Form.bulk_subst] at h ⊢
+            apply Or.inl
+            exact occurs_list_noms.mp h
+        | cons h_old t_old =>
+            simp [Form.bulk_subst] at eq_len h ⊢
+            have := ih eq_len h
+            apply Or.elim this
+            . intro hyp
+              clear this ih
+              cases t_new
+              . have := List.length_eq_zero.mp (Eq.symm (Eq.subst eq_len (@List.length_nil NOM)))
+                simp [this, Form.bulk_subst] at h ⊢
+                apply Or.elim (list_noms_subst (occurs_list_noms.mp h))
+                . intro c1
+                  simp [c1]
+                . intro c2
+                  exact Or.inr c2
+              . cases t_old
+                . simp at eq_len
+                . simp [Form.bulk_subst] at hyp ⊢
+                  have ⟨a, b⟩ := hyp
+                  apply Or.elim (list_noms_subst b)
+                  . intro c1
+                    apply Or.inl
+                    simp [c1, a]
+                  . intro c2
+                    simp [c2]
+            . intro hyp
+              clear this ih
+              apply Or.inr
+              apply Or.inr
+              assumption
+
+  -- FORM.DBL_LIST_NOMS DOESN'T HAVE THIS PROPERTY
+  theorem nocc_bulk {l_new l_old : List NOM} {φ : Form} (eq_len : l_new.length = l_old.length) : ((i ∉ φ.list_noms ∨ i ∈ l_old) ∧ i ∉ l_new) → nom_occurs i (φ.bulk_subst l_new l_old) = false := by
+    rw [contraposition]
+    simp [-implication_disjunction]
+    intro h1 h2
+    apply Or.elim (occ_bulk eq_len h1)
+    . simp
+    . simp [h2]
+
+  def map_odd : ℕ → NOM → NOM := λ off => λ h => ⟨h.letter*2 + off + (1 - off % 2)⟩ 
+  def map_odd_inv : ℕ → NOM → NOM := λ off => λ h => ⟨(h.letter - (1 - off % 2) - off)/2⟩
+
+  theorem map_odd_inv_is_inv : map_odd_inv off (map_odd off i) = i := by
+    simp [map_odd_inv, map_odd]
+
+  theorem map_odd_ge  : map_odd off i ≥ ⟨off⟩ := by
+    simp [map_odd, NOM.le, Nat.add_comm, Nat.add_assoc]
+
+  def Form.mapping1 : Form → Form := λ φ => φ.bulk_subst (φ.list_noms.map (map_odd φ.new_nom.letter)) φ.list_noms
+  def Form.mapping2 : Form → Form := λ φ =>
+    φ.mapping1.bulk_subst (φ.mapping1.list_noms.map (map_odd_inv φ.new_nom.letter)) φ.mapping1.list_noms
+
+  theorem mapping_inv {φ : Form} : φ.mapping1.mapping2 = φ := by
+    unfold Form.mapping1 Form.mapping2
+    admit 
+
+  theorem mapping1nocc : ∀ i : NOM, i ∈ (φ.list_noms.map (map_odd φ.new_nom.letter)) → nom_occurs i φ = false := by
+    intro i hmem
+    apply ge_new_nom_is_new
+    simp at hmem
+    have ⟨a, p1, _⟩ := hmem
+    have := @map_odd_ge φ.new_nom.letter a
+    rw [p1] at this
+    exact this
+
+  def all_nocc : List NOM → Form → Prop := λ l => λ φ =>  ∀ i, i ∈ l → nom_occurs i φ = false
+
+/-
+  theorem nom_nom_nom_subst {i j a : NOM} (h : nom_occurs i φ = false ∧ nom_occurs j φ = false) : φ[j // a] = φ[i // a][j // i] := by
+    induction φ <;> simp [nom_subst_nom, nom_occurs, *, -implication_disjunction] at *
+    . split <;> simp [nom_subst_nom, Ne.symm, h]
+    . simp [h] at *
+      apply And.intro
+      repeat assumption
+    repeat { simp [h.left, h.right] at *; assumption  }
+
+  -- ((φ[a // b]).bulk_subst l1 l2)
+
+  theorem remember {φ : Form} {h_new : NOM} : (φ.bulk_subst (h_old :: t) t_orig)[h_new // h_old] = φ.bulk_subst (h_new :: t) t_orig := sorry
+
+  theorem triangle_subst {φ : Form} (l₁ l₂ : List NOM) (h1: all_nocc l₁ φ ∧ all_nocc l₂ φ) (h2 : l₁ ≠ [] ∧ l₂ ≠ []) :
+      φ.bulk_subst l₁ φ.list_noms = (φ.bulk_subst l₂ φ.list_noms).bulk_subst l₁ l₂ := by
+      induction φ.list_noms generalizing φ l₁ l₂ with
+      | nil => simp [Form.bulk_subst]; admit
+      | cons h_orig t_orig ih =>
+          cases l₁ with
+          | nil => simp at h2
+          | cons head₁ tail₁ =>
+              cases l₂ with
+              | nil => simp at h2
+              | cons head₂ tail₂ =>
+                  rw [Form.bulk_subst, Form.bulk_subst, remember, Form.bulk_subst]
+                  have nih := @ih (φ[head₁ // h_orig])
+                  clear ih
+
+                  --conv at ih => rhs; rw [Form.bulk_subst, remember]
+                  
+                  --simp only [Form.bulk_subst] at ih ⊢
+                  admit
+      /-
+      cases l₁ with
+      | nil => simp at h5
+      | cons h₁ t₁ =>
+          cases l₂ with
+          | nil => simp at h5
+          | cons h₂ t₂ =>
+              simp [all_nocc, -implication_disjunction] at h1 h2
+              clear h5
+              revert h3 h4
+              cases φ.list_noms
+              . simp [Form.bulk_subst, -implication_disjunction]
+                intro h3 h4
+                rw [h3, h4]
+                admit
+              . simp [Form.bulk_subst, -implication_disjunction]
+                intro h3 h4
+                rw [h4]
+                admit
+        -/
+-/
+/-
+  def Form.map_odd_list : Form → List NOM → ℕ → Form 
+  | φ, [], _            => φ
+  | φ, h :: t, offset   => 
+      φ[map_odd_n offset h // h].map_odd_list t offset
+
+  def Form.map_odd      : Form → Form := λ φ => φ.map_odd_list φ.nominals φ.new_nom.letter
+
+  theorem eddie (φ : Form) : φ.map_odd.nominals = φ.nominals.map (map_odd_n φ.new_nom.letter) := by
+    induction φ with
+    | impl ψ χ ih1 ih2 =>
+        simp [Form.map_odd]        
+        admit
+    | _ => admit 
+
+  theorem helper {φ : Form} : ∀ i : NOM, nom_occurs i φ.map_odd → i ≥ φ.new_nom := by
+    intro i
+    rw [Form.map_odd]
+    have h : φ.nominals = [] ↔ ∀ i : NOM, nom_occurs i φ = false := hmm φ
+    revert h
+    induction φ.nominals generalizing φ with
+    | nil =>
+        simp only [true_iff, Form.map_odd_list, ge_iff_le]
+        intro a b
+        exfalso
+        have := Eq.mpr (Bool.eq_false_eq_not_eq_true (nom_occurs i φ)) (a i)
+        contradiction
+    | cons h t ih =>
+        let ψ : Form := sorry
+        have : t = ψ.nominals := sorry
+        rw [this] at ih
+        have new_ih := ih (hmm ψ)
+        clear ih
+        simp only [Form.map_odd_list]
+        intro c hocc
+        clear c
+        admit
+
+  def Form.double_list : Form → List NOM → Form
+  | φ, []       => φ
+  | φ, h :: t   => φ [NOM.mk (h.letter * 2) // h].double_list t
+
+  def Form.half_list : Form → List NOM → Form
+  | φ, []       => φ
+  | φ, h :: t   => φ [NOM.mk (h.letter / 2) // h].double_list t
+
+  def Form.double  : Form → Form   :=   λ φ => φ.double_list (φ.nominals)
+  def Form.half    : Form → Form   :=   λ φ => φ.half_list (φ.nominals)
+
+--  notation:150 φ "*2" => Form.double φ
+--  notation:150 φ "/2" => Form.half φ
+
+  def Set.double : Set Form → Set Form := λ Γ => {Form.double φ | φ ∈ Γ}
+  def Set.half   : Set Form → Set Form := λ Γ => {Form.half φ | φ ∈ Γ}
+
+  def Form.double_n : Form → ℕ → Form
+  | φ, 0         => φ
+  | φ, n+1       => (nom_subst_nom φ ⟨2*(n+1)⟩ ⟨n+1⟩).double_n n
+
+  def Form.double'  : Form → Form   := λ φ => φ.double_n φ.new_nom.letter
+
+  def Form.double''  : Form → Form   := λ φ =>
+    loop φ φ.new_nom.letter
+  where
+    loop : Form → ℕ → Form
+    | φ, 0      => φ
+    | φ, n+1    => loop (nom_subst_nom φ ⟨2*n⟩ ⟨n⟩) n
+
+
+  #eval (NOM.mk 3 ⋁ NOM.mk 6).double''
+--  notation:150 Γ "*2" => Set.double Γ 
+--  notation:150 Γ "/2" => Set.half Γ 
+-/
+end NominalSubstitution
 
 section IteratedModalities
 
