hybrid/Proof.lean
@@ -1,42 +1,38 @@
 import Hybrid.Form
+import Hybrid.Tautology
 
 inductive Proof : Form → Prop where
   -- Deduction rules:
 
-  -- if φ can be deduced from Γ, then so can ∀ v, φ
-  -- todo: add restrictions 
-  | general {φ : Form}:
+  -- if φ is a theorem, ∀ v, φ is a theorem
+  | general {φ : Form} (v : SVAR):
         Proof φ → Proof (all v, φ)
 
-  -- if φ is a theorem, □ φ can be deduced from any Γ 
-  | necess {φ : Form}:
+  -- if φ is a theorem, □ φ is a theorem 
+  | necess (φ : Form):
         Proof φ → Proof (□ φ)
 
   -- modus ponens:
-  | ponens {φ ψ : Form}:
+  | mp {φ ψ : Form}:
         Proof (φ ⟶ ψ) → Proof φ → Proof ψ
 
-  -- add all instances of propositional tautologies...
-  | tautology₁ {φ ψ : Form}:
-        Proof (φ ⟶ (ψ ⟶ φ))
-  | tautology₂ {φ ψ χ : Form}:
-        Proof ((φ ⟶ (ψ ⟶ χ)) ⟶ ((φ ⟶ ψ) ⟶ (φ ⟶ χ))) 
-  | tautology₃ {φ ψ : Form}:
-        Proof ((∼φ ⟶ ∼ψ) ⟶ (ψ ⟶ φ))
+  -- All propositional tautologies
+  | tautology {φ : Form}:
+        Tautology φ → Proof φ
 
   -- Axioms for modal + hybrid logic:
   -- distribution schema (axiom K)
   | ax_k {φ ψ : Form}:
         Proof (□ (φ ⟶ ψ) ⟶ (□ φ ⟶ □ ψ))
 
-  | ax_q1 {φ ψ : Form} {v : SVAR} (p : ¬ is_free v φ):
+  | ax_q1 (φ ψ : Form) {v : SVAR} (p : is_free v φ = false):
         Proof ((all v, φ ⟶ ψ) ⟶ (φ ⟶ all v, ψ))
 
   -- two different instances of Axiom Q2: one for SVAR, one for NOM
-  | ax_q2_svar {φ : Form} (v : SVAR) (s : SVAR) (p : is_substable φ s v):
+  | ax_q2_svar (φ : Form) (v s : SVAR) (p : is_substable φ s v):
       Proof ((all v, φ) ⟶ φ[s // v])
 
-  | ax_q2_nom {φ : Form} (v : SVAR) (s : NOM):
+  | ax_q2_nom (φ : Form) (v : SVAR) (s : NOM):
       Proof ((all v, φ) ⟶ φ[s // v])
 
   | ax_name (v : SVAR):
@@ -48,7 +44,8 @@ inductive Proof : Form → Prop where
   | ax_brcn {φ : Form} {v : SVAR}:
       Proof ((all v, □ φ) ⟶ (□ all v, φ))
 
-def SyntacticConsequence (Γ : List Form) (φ : Form) : Prop := Proof ((conjunction Γ) ⟶ φ)  
+def SyntacticConsequence (Γ : Set Form) (φ : Form) : Prop := ∃ L, Proof ((conjunction Γ L) ⟶ φ)  
+
 
 prefix:500 "⊢"  => Proof
 infix:500 "⊢"   => SyntacticConsequence
@@ -56,4 +53,12 @@ infix:500 "⊢"   => SyntacticConsequence
 notation "⊬" φ    => ¬ (Proof φ)
 notation Γ "⊬" φ  => ¬ (SyntacticConsequence Γ φ) 
 
-def consistent_set (Γ : List Form) := Γ ⊬ ⊥ 
+def Set.consistent (Γ : Set Form) := Γ ⊬ ⊥
+
+def Set.MCS (Γ : Set Form) := Γ.consistent ∧ (∀ φ : Form, (¬φ ∈ Γ) → (Γ ∪ {φ}) ⊢ ⊥)
+
+def Set.witnessed (Γ : Set Form) : Prop := ∀ {φ : Form},
+  φ ∈ Γ → 
+    match φ with 
+      | ex x, ψ => ∃ i : NOM, ((ex x, ψ) ⟶ ψ[i // x]) ∈ Γ 
+      | _   => φ ∈ Γ
