hybrid/Soundness.lean
@@ -5,60 +5,51 @@ import Hybrid.Util
 open Classical
 
 section Lemmas
-  theorem generalize_bound {φ : Form} {v : SVAR} {M : Model} {s : M.W} {g : I M.W} (h1 : ¬is_free v φ) (h2 : (M,s,g) ⊨ φ) : ((M,s,g) ⊨ all v, φ) :=
+  theorem generalize_not_free (h1 : is_free v φ = false) : ⊨ (φ ⟶ (all v, φ)) := by
+    intro M s g
+    intro h2
     match φ with
-    | Form.bttm   => False.elim h2
-    | Form.prop p => by
+    | Form.bttm   => exact False.elim h2
+    | Form.prop p =>
         simp at h2
         rw [Sat]
         intros
         exact h2
-    | Form.svar _ =>
-        have not_h1 : is_free v (Form.svar _) := trivial
-        False.elim (h1 not_h1)
+    | Form.svar x =>
+        simp only [is_free, beq_eq_false_iff_ne, ne_eq] at h1 
+        intro _ var
+        exact Eq.trans h2 (Eq.symm (var x h1))
     | Form.nom _ =>
-        have not_h1 : is_free v (Form.nom _) := trivial
-        False.elim (h1 not_h1)
-    | Form.impl ψ χ => by
+        intro _ _
+        exact h2
+    | Form.impl ψ χ =>
         rw [Sat]
-        rw [is_free, negated_disjunction] at h1
+        simp only [is_free, Bool.or_eq_false_eq_eq_false_and_eq_false] at h1 
         rw [Sat] at h2
         intros g' variant antecedent
         have sym_variant := is_variant_symm.mp variant
         -- apply the induction hypothesis:
-        have by_ind_hyp := generalize_bound h1.left antecedent
-        have by_mp_ind  := generalize_bound h1.right (h2 (by_ind_hyp g sym_variant))
+        have by_ind_hyp := generalize_not_free h1.left M s g' antecedent
+        have by_mp_ind  := generalize_not_free h1.right M s g (h2 (by_ind_hyp g sym_variant))
         exact by_mp_ind g' variant
-    | Form.box ψ    => by
+    | Form.box ψ    =>
         rw [is_free] at h1
         intros g' variant s' is_neigh
-        exact generalize_bound h1 (h2 s' is_neigh) g' variant
-    | Form.bind u ψ => by
-        -- ugly and convoluted
-        -- can you rewrite this?
-        rw [is_free] at h1
-        have h1_rw : (u = v ∨ ¬is_free v ψ) :=
-          byContradiction
-          (λ nh1_rw => by
-            simp at nh1_rw
-            have nh1 : if u = v then False else is_free v ψ :=
-              match (instDecidableEqSVAR u v) with
-              | isTrue u_is_v => False.elim (nh1_rw.left u_is_v)
-              | isFalse _ => nh1_rw.right
-            exact False.elim (h1 nh1)
-          )
-        ---
-        apply Or.elim h1_rw
+        exact generalize_not_free h1 M s' g (h2 s' is_neigh) g' variant
+    | Form.bind u ψ =>
+        simp only [is_free, Bool.and_eq_false_eq_eq_false_or_eq_false] at h1  
+        apply Or.elim h1
         . intro u_is_v
+          simp only [bne, Bool.not_eq_false', beq_iff_eq] at u_is_v 
           rw [u_is_v]
           rw [u_is_v] at h2
           intros g' variant1 g'' variant2
           have variant3 := is_variant_trans variant2 variant1
           exact h2 g'' variant3
-        . intro bound_in_ψ
+        . intro nfree_in_ψ
           rw [bind_comm]
           intros g' variant_u
-          exact generalize_bound bound_in_ψ (h2 g' variant_u)
+          exact generalize_not_free nfree_in_ψ M s g' (h2 g' variant_u)
 
   theorem svar_substitution {φ : Form} {x y : SVAR} {M : Model} {s : M.W} {g g' : I M.W} 
   (h_subst : is_substable φ y x) (h_var : is_variant g g' x) (h_which_var : g' x = g y) :
@@ -83,6 +74,7 @@ section Lemmas
             rw [Sat, ←(h_var z (Ne.symm z_x))] at h
             exact h
     | impl ψ χ ind_hyp_1 ind_hyp_2 =>
+        simp only [is_substable, Bool.and_eq_true] at h_subst 
         have by_ind_hyp_1 := (@ind_hyp_1 s g) h_subst.left h_var h_which_var
         have by_ind_hyp_2 := (@ind_hyp_2 s g) h_subst.right h_var h_which_var
         apply Iff.intro
@@ -100,79 +92,77 @@ section Lemmas
           have by_ind_hyp := (@ind_hyp s' g) h_subst h_var h_which_var
           exact by_ind_hyp.mpr (h1 s' s_R_s')
     | bind v ψ ind_hyp =>
-        by_cases x_free : is_free x ψ
-        . by_cases x_v : x = v
-          . -- all x, ψ             and       x is free in ψ
-            have x_bound : ¬is_free x (all v, ψ) :=
-              by conv => rhs rhs lhs rw [←x_v] ; exact not_bound_when_quantified
-            apply Iff.intro
-            . intro h1
-              conv at h1 => rhs ; rw [subst_bound_var x_bound]
-              exact (generalize_bound x_bound h1) g' (is_variant_symm.mp h_var)
-            . intro h1
-              conv => rhs ; rw [subst_bound_var x_bound, ←x_v]
-              rw [←x_v] at h1
-              rw [←x_v] at x_bound
-              exact (generalize_bound x_bound h1) g h_var
-          . by_cases y_v : y = v
-            . -- all y, ψ          and       x is free in ψ
-              unfold is_substable at h_subst
-              rw [if_neg (double_negation.mpr x_free), if_neg (double_negation.mpr y_v)] at h_subst
-              exact False.elim h_subst
-            . --  all v, ψ  (v ≠ x and v ≠ y) and x is free in ψ
-              --
-              -- simplify h_subst to is_substable ψ y x :
-              unfold is_substable at h_subst
-              rw [if_neg (double_negation.mpr x_free), if_pos y_v] at h_subst
-              -- proof:
+        cases x_free : is_free x ψ with
+        | true =>
+            by_cases x_v : x = v
+            . -- all x, ψ             and       x is free in ψ
+              have x_nfree : is_free x (all v, ψ) = false := by
+                simp only [is_free, x_v, bne_self_eq_false, Bool.false_and]
               apply Iff.intro
               . intro h1
-                -- step one: turn
-                --  (M,s,g)⊨(all v, ψ)[y//x] into
-                --  (M,s,g)⊨all v, ψ[y//x]
-                unfold subst_svar at h1
-                rw [if_neg x_v] at h1
-                -- step two
-                intro f' f'_var_g'_v
-                -- Here's the fun part. We're going to apply the
-                --  variant mirror property to f' and g', to obtain
-                --  an interpretation f that is a v-variant of g and 
-                --  also an x-variant of f'.
-                -- Since f is a v-variant of g and we have (M,s,g)⊨all v, ψ[y//x],
-                --  we'll obtain (M,s,f)⊨ψ[y//x].
-                -- From there, we'll apply the induction hypothesis to f and f'
-                --  and prove the goal.
-                have exists_mirror := variant_mirror_property g g' f' h_var (is_variant_symm.mp f'_var_g'_v)
-                match exists_mirror with
-                | ⟨f, f_var_g_v, f_var_f'_x⟩ =>
-                    have t1 : f' x = f y := by
-                      rw [show f y = g y from Eq.symm (f_var_g_v y (Ne.symm (Ne.intro y_v)))]
-                      rw [show f' x = g' x from f'_var_g'_v x (Ne.symm (Ne.intro x_v))]
-                      assumption
-                    have t2 : (M,s,f) ⊨ ψ[y//x] := h1 f (is_variant_symm.mpr f_var_g_v)
-                    exact (@ind_hyp s f f' h_subst f_var_f'_x t1).mp t2
+                rw [(subst_notfree_var x_nfree).left] at h1
+                exact (generalize_not_free x_nfree M s g h1) g' (is_variant_symm.mp h_var)
               . intro h1
-                -- do the same thing backwards, basically
-                unfold subst_svar
-                rw [if_neg x_v]
-                intro f f_var_g_v
-                have exists_mirror := variant_mirror_property f g g' f_var_g_v h_var
-                match exists_mirror with
-                | ⟨f', f_var_f'_x, f'_var_g'_v⟩ =>
-                  have t1 : f' x = f y := by
-                      rw [show f y = g y from f_var_g_v y (Ne.symm (Ne.intro y_v))]
-                      rw [show f' x = g' x from f'_var_g'_v x (Ne.symm (Ne.intro x_v))]
-                      assumption
-                  have t2 : (M,s,f') ⊨ ψ := h1 f' f'_var_g'_v
-                  exact (@ind_hyp s f f' h_subst f_var_f'_x t1).mpr t2
-        . have x_bound : ¬is_free x (all v, ψ) := preserve_boundness x_free
-          apply Iff.intro
-          . intro h2 g'' v_variant
-            conv at h2 => rhs ; rw [subst_bound_var x_bound]
-            exact ((generalize_bound x_bound h2) g' (is_variant_symm.mp h_var)) g'' v_variant
-          . intro h2
-            conv => rhs ; rw [subst_bound_var x_bound]
-            exact (generalize_bound x_bound h2) g h_var
+                conv => rhs ; rw [(subst_notfree_var x_nfree).left, ←x_v]
+                rw [←x_v] at h1
+                rw [←x_v] at x_nfree
+                exact (generalize_not_free x_nfree M s g' h1) g h_var
+            . by_cases y_v : y = v
+              . -- all y, ψ          and       x is free in ψ
+                -- contradiction with h_subst:
+                simp only [is_substable, x_free, beq_iff_eq, y_v,
+                  bne_self_eq_false, Bool.false_and, ite_false] at h_subst   
+              . --  all v, ψ  (v ≠ x and v ≠ y) and x is free in ψ
+                simp only [is_substable, x_free, beq_iff_eq, bne, ite_false, Bool.and_eq_true, Bool.not_eq_true',
+                  beq_eq_false_iff_ne, ne_eq, Ne.symm y_v, not_false_eq_true, true_and] at h_subst 
+                -- proof:
+                apply Iff.intro
+                . intro h1
+                  -- step one: turn
+                  --  (M,s,g)⊨(all v, ψ)[y//x] into
+                  --  (M,s,g)⊨all v, ψ[y//x]
+                  simp only [subst_svar, if_neg x_v] at h1
+                  -- step two
+                  intro f' f'_var_g'_v
+                  -- Here's the fun part. We're going to apply the
+                  --  variant mirror property to f' and g', to obtain
+                  --  an interpretation f that is a v-variant of g and 
+                  --  also an x-variant of f'.
+                  -- Since f is a v-variant of g and we have (M,s,g)⊨all v, ψ[y//x],
+                  --  we'll obtain (M,s,f)⊨ψ[y//x].
+                  -- From there, we'll apply the induction hypothesis to f and f'
+                  --  and prove the goal.
+                  have exists_mirror := variant_mirror_property g g' f' h_var (is_variant_symm.mp f'_var_g'_v)
+                  match exists_mirror with
+                  | ⟨f, f_var_g_v, f_var_f'_x⟩ =>
+                      have t1 : f' x = f y := by
+                        rw [show f y = g y from Eq.symm (f_var_g_v y (Ne.symm (Ne.intro y_v)))]
+                        rw [show f' x = g' x from f'_var_g'_v x (Ne.symm (Ne.intro x_v))]
+                        assumption
+                      have t2 : (M,s,f) ⊨ ψ[y//x] := h1 f (is_variant_symm.mpr f_var_g_v)
+                      exact (@ind_hyp s f f' h_subst f_var_f'_x t1).mp t2
+                . intro h1
+                  -- do the same thing backwards, basically
+                  simp only [subst_svar, if_neg x_v]
+                  intro f f_var_g_v
+                  have exists_mirror := variant_mirror_property f g g' f_var_g_v h_var
+                  match exists_mirror with
+                  | ⟨f', f_var_f'_x, f'_var_g'_v⟩ =>
+                    have t1 : f' x = f y := by
+                        rw [show f y = g y from f_var_g_v y (Ne.symm (Ne.intro y_v))]
+                        rw [show f' x = g' x from f'_var_g'_v x (Ne.symm (Ne.intro x_v))]
+                        assumption
+                    have t2 : (M,s,f') ⊨ ψ := h1 f' f'_var_g'_v
+                    exact (@ind_hyp s f f' h_subst f_var_f'_x t1).mpr t2
+        | false =>
+            have x_nfree : is_free x (all v, ψ) = false := preserve_notfree x v x_free
+            apply Iff.intro
+            . intro h2 g'' v_variant
+              conv at h2 => rhs ; rw [(subst_notfree_var x_nfree).left]
+              exact ((generalize_not_free x_nfree M s g h2) g' (is_variant_symm.mp h_var)) g'' v_variant
+            . intro h2
+              conv => rhs ; rw [(subst_notfree_var x_nfree).left]
+              exact (generalize_not_free x_nfree M s g' h2) g h_var
     | _        => simp
 
     theorem nom_substitution {φ : Form} {x : SVAR} {i : NOM} {M : Model} {s : M.W} {g g' : I M.W}
@@ -202,14 +192,18 @@ section Lemmas
       | impl ψ χ ih_1 ih_2 =>
           have ih_1 := @ih_1 s g g' h_var h_which_var
           have ih_2 := @ih_2 s g g' h_var h_which_var
-          conv => lhs rhs rw[subst_nom]
+          conv => lhs
+                  rhs
+                  rw [subst_nom]
           apply Iff.intro
           . intro h1 antecedent
             exact ih_2.mp (h1 (ih_1.mpr antecedent))
           . intro h2 antecedent
             exact ih_2.mpr (h2 (ih_1.mp antecedent))
       | box ψ ih =>
-          conv => lhs rhs rw[subst_nom]
+          conv => lhs
+                  rhs
+                  rw [subst_nom]
           apply Iff.intro
           . intro h1 s' s_R_s'
             have ih := @ih s' g g' h_var h_which_var
@@ -218,7 +212,9 @@ section Lemmas
             have ih := @ih s' g g' h_var h_which_var
             exact ih.mpr (h2 s' s_R_s')
       | bind y ψ ih =>
-          conv => lhs rhs rw[subst_nom]
+          conv => lhs
+                  rhs
+                  rw [subst_nom]
           by_cases x_y : x = y
           . rw [if_pos x_y]
             apply Iff.intro
@@ -322,28 +318,65 @@ section Lemmas
   (((M,s,g) ⊨ Form.svar v) → (∀ r : M.W, ((M,r,g) ⊨ Form.svar v) → r = s)) := by
     intro h1 r h2
     rw [h2, h1]
-
 end Lemmas
+
+section Tautologies
+  -- Todo: find a a proof of soundness for tautologies that doesn't rely
+  -- on Sat's decidability.  
+  noncomputable def model_val_func (M : Model) (s : M.W) (g : I M.W) : Form → Bool
+    | Form.bttm     => false
+    | Form.prop p   => ite ((M,s,g) ⊨ p) true false
+    | Form.nom  i   => ite ((M,s,g) ⊨ i) true false
+    | Form.svar x   => ite ((M,s,g) ⊨ x) true false
+    | Form.impl ψ χ => ¬(model_val_func M s g ψ = true) ∨ model_val_func M s g χ = true
+    | Form.box ψ    => ite ((M,s,g) ⊨ □ψ) true false
+    | Form.bind x ψ => ite ((M,s,g) ⊨ all x, ψ) true false
+
+  noncomputable def model_eval (M : Model) (s : M.W) (g : I M.W) : Eval :=
+      let f := model_val_func M s g
+      have p1 : f ⊥ = false := by simp [model_val_func]
+      have p2 : ∀ φ ψ : Form, (f (φ ⟶ ψ) = true) ↔ (¬(f φ) = true ∨ (f ψ) = true) := λ φ ψ : Form => by simp [model_val_func] 
+      ⟨f, p1, p2⟩
+
+  theorem model_eval_equiv (M : Model) (s : M.W) (g : I M.W) (f : Form → Bool) (h : f = model_val_func M s g) : ∀ φ : Form, ((M,s,g) ⊨ φ) ↔ f φ = true := by
+    intro φ
+    induction φ with
+    | impl _ _ ih1 ih2 =>
+        simp [h, model_val_func] at ih1
+        simp [h, model_val_func] at ih2
+        simp [h, model_val_func, ih1, ih2]
+    | box _ ih  =>
+        simp [h, model_val_func] at ih
+        simp [h, model_val_func, ih, -Sat]
+    | bind _ _ ih  =>
+        simp [h, model_val_func] at ih
+        simp [h, model_val_func, ih, -Sat]
+    | _  =>
+        simp [h, model_val_func]
+
+  theorem taut_sound : Tautology φ → ⊨ φ := by
+    rw [contraposition (Tautology φ) (⊨ φ), Valid, Tautology]
+    conv =>
+      rw [negated_universal, negated_universal]
+      congr
+      . rhs; intro M; rw [negated_universal]; rhs; intro s; rw [negated_universal]; rhs; intro g; rw [←neg_sat]
+      . rhs; intro e; rw [Bool.not_eq_true, ←e_neg]
+    intro h
+    match h with
+    | ⟨M, s, g, hw⟩ =>
+        let eval := model_eval M s g
+        exists eval
+        have : (eval.f) = (model_val_func M s g) := by simp [model_eval]
+        have equiv := model_eval_equiv M s g eval.f this (∼φ)
+        rw [←equiv]
+        exact hw
+end Tautologies
 
 theorem WeakSoundness : (⊢ φ) → (⊨ φ) := by
   intro pf
   induction pf with
-  | tautology₁ =>
-      intro _ _ _ phi _
-      exact phi
 
-  | tautology₂ =>
-      intro _ _ _ h1 h2 h3
-      exact (h1 h3) (h2 h3)
-
-  | tautology₃ =>
-      intro _ _ _ h1 h2
-      rw [Sat, neg_sat, implication_disjunction, double_negation] at h1
-      apply Or.elim h1
-      . intro
-        assumption
-      . intro h3
-        exact False.elim (h3 h2)
+  | tautology h => exact taut_sound h
 
   | ax_k =>
       intro (M : Model) (s : M.W) (g : I M.W)
@@ -351,11 +384,11 @@ theorem WeakSoundness : (⊢ φ) → (⊨ φ) := by
       intro nec_impl nec_phi (s' : M.W) (rel : M.R s s')
       exact (nec_impl s' rel) (nec_phi  s' rel)
 
-  | ax_q1 p =>
-      intro _  g _ h1 h2 g' variant
-      exact (h1 g' variant) ((generalize_bound p h2) g' variant)
+  | ax_q1 _ _ p =>
+      intro M s g h1 h2 g' variant
+      exact (h1 g' variant) ((generalize_not_free p M s g h2) g' variant)
 
-  | ax_q2_svar x y h_subst =>
+  | ax_q2_svar _ x y h_subst =>
       intro (M : Model) (s : M.W) (g : I M.W)
       intro h
       -- let's build an explicit x-variant of g, named g'
@@ -369,7 +402,7 @@ theorem WeakSoundness : (⊢ φ) → (⊨ φ) := by
       -- now the goal becomes immediately provable
       exact h g' (is_variant_symm.mp h_var)
   
-  | ax_q2_nom x i =>
+  | ax_q2_nom _ x i =>
       intro (M : Model) (s : M.W) (g : I M.W)
       intro h
       let g' : I M.W := λ v => ite (v ≠ x) (g v) (M.Vₙ i)
@@ -410,18 +443,28 @@ theorem WeakSoundness : (⊢ φ) → (⊨ φ) := by
       intro M s g (h : (M,s,g) ⊨ all v, □φ) s' sRs' g' g_var_g'_v
       exact (h g' g_var_g'_v) s' sRs'
 
-  | general _ ih =>
+  | general _ _ ih =>
       intro M s _ g' _
       exact ih M s g'
 
-  | necess _ ih =>
+  | necess _ _ ih =>
       intro M _ g s' _
       exact ih M s' g
 
-  | ponens _ _ ih_maj ih_min =>
+  | mp _ _ ih_maj ih_min =>
       intro M s g
       exact (ih_maj M s g) (ih_min M s g)
 
 theorem Soundness : (Γ ⊢ φ) → (Γ ⊨ φ) := by
-  rw [SyntacticConsequence, SemanticConsequence]
-  exact @WeakSoundness (conjunction Γ⟶φ)
+  rw [SyntacticConsequence]
+  intro h
+  apply SetEntailment
+  match h with
+  | ⟨L, conseq⟩ =>
+    have := (@WeakSoundness (conjunction Γ L⟶φ)) conseq
+    exact ⟨L, this⟩
+
+#print axioms Soundness
+#check propext
+#check Classical.choice
+#check Quot.sound
